Move proof of trivial_deterministic into own file

src/ReactorModel/Determinism/Execution.lean
@@ -1,35 +1,9 @@
 import ReactorModel.Determinism.ExecutionStep
+import ReactorModel.Determinism.Trivial
 
 open Classical 
 
 namespace Execution
-
--- This is only used for the proof of `trivial_deterministic`.
-inductive AdvanceTag.RTC : State → State → Type
-  | refl : RTC s s
-  | trans : (s₁ ⇓- s₂) → (RTC s₂ s₃) → RTC s₁ s₃   
-
--- This is only used for the proof of `trivial_deterministic`.
-theorem AdvanceTag.RTC.deterministic 
-  (a₁ : AdvanceTag.RTC s s₁) (a₂ : AdvanceTag.RTC s s₂) (ht : s₁.tag = s₂.tag) : s₁ = s₂ := by
-  induction a₁ <;> cases a₂
-  case refl.refl                       => rfl
-  case' refl.trans a _, trans.refl _ a => exact absurd ht a.tag_ne
-  case trans.trans a₁ _ hi _ a₂ c₂     => exact hi (a₂.determinisic a₁ ▸ c₂) ht
-
--- This is only used for the proof of `trivial_deterministic`.
-def trivial_erase_exec_steps [State.Trivial s₁] : (s₁ ⇓* s₂) → AdvanceTag.RTC s₁ s₂
-  | refl => .refl
-  | step (.advance a) e' => 
-    have := a.preserves_Trivial -- TODO: Make this work via type class inference.
-    .trans a e'.trivial_erase_exec_steps
-  | step (.close e) e' => 
-    have := e.preserves_Trivial -- TODO: Make this work via type class inference.
-    e.trivial_eq ▸ e'.trivial_erase_exec_steps
-
-theorem trivial_deterministic [trivial : State.Trivial s] 
-    (e₁ : s ⇓* s₁) (e₂ : s ⇓* s₂) (ht : s₁.tag = s₂.tag) : s₁ = s₂ :=
-  AdvanceTag.RTC.deterministic e₁.trivial_erase_exec_steps e₂.trivial_erase_exec_steps ht
 
 theorem tag_le : (s₁ ⇓* s₂) → s₁.tag ≤ s₂.tag
   | refl      => le_refl _
