src/ReactorModel/Determinism/InstExecution.lean
@@ -3,51 +3,11 @@ import ReactorModel.Determinism.InstStep
 open Classical
 
 namespace Execution
+namespace InstExecution
 
 open State (Closed)
 
-theorem InstExecution.tag_eq : (s₁ ⇓ᵢ* s₂) → s₁.tag = s₂.tag
-  | refl => rfl
-  | trans e e' => e.exec.preserves_tag.trans e'.tag_eq
-
-theorem InstExecution.preserves_ctx_past_future :
-  (s₁ ⇓ᵢ* s₂) → ∀ g, g ≠ s₁.tag → s₁.ctx.processedRcns g = s₂.ctx.processedRcns g := by
-  intro h g hg
-  induction h
-  case refl => rfl
-  case trans s₁ _ sₘ he _ hi =>
-    rw [InstExecution.tag_eq $ trans he refl] at hg
-    exact (he.exec.preserves_ctx_past_future _ hg).trans $ hi hg
-    
-  /-
-  
-  ext1; ext1 g
-  have hc₁₂ := hc₁.rcns_eq hc₂
-  cases hc₁ with | mk e₁ hc₁ => 
-  cases hc₂ with | mk e₂ hc₂ => 
-  by_cases hg : g = s.tag
-  case pos => 
-    have h₁ := hc₁ |> Option.some_inj.mpr
-    have h₂ := hc₂ |> Option.some_inj.mpr
-    rw [Context.progress_def] at h₁ h₂
-    simp only [←e₁.tag_eq, ←e₂.tag_eq, ←hg] at h₁ h₂
-    simp only [h₁, h₂, hc₁₂]
-  case neg => simp only [←e₁.preserves_ctx_past_future g hg, e₂.preserves_ctx_past_future g hg]
-  -/
-
-theorem InstExecution.ctx_eq (e : s₁ ⇓ᵢ* s₂) : s₂.ctx = s₁.ctx.process e.rcns :=
-  sorry
-
-theorem InstExecution.mem_rcns_iff (e : s₁ ⇓ᵢ* s₂) (rcn : ID) : 
-  rcn ∈ e.rcns ↔ (rcn ∈ s₂.progress ∧ rcn ∉ s₁.progress) := by
-  sorry
-
-theorem InstExecution.preserves_rcns {i : ID} :
-  (s₁ ⇓ᵢ* s₂) → (s₁.rtr.obj? .rcn i = s₂.rtr.obj? .rcn i)
-  | refl => rfl
-  | trans h₁ₘ hₘ₂ => h₁ₘ.exec.preserves_rcns.trans hₘ₂.preserves_rcns
-
-theorem InstExecution.rcns_unprocessed : 
+theorem rcns_unprocessed : 
   (e : s₁ ⇓ᵢ* s₂) → ∀ rcn ∈ e.rcns, rcn ∉ s₁.progress := by
   intro h rcn hr
   induction h
@@ -67,11 +27,11 @@ theorem InstExecution.rcns_unprocessed :
       specialize hi h
       exact ((not_or _ _).mp $ (mt h₁.mem_progress.mpr) hi).right
 
-theorem InstExecution.rcns_nodup : (e : s₁ ⇓ᵢ* s₂) → List.Nodup e.rcns
+theorem rcns_nodup : (e : s₁ ⇓ᵢ* s₂) → List.Nodup e.rcns
   | refl => List.Nodup.nil
   | trans h₁ h₂ => List.nodup_cons.mpr $ ⟨(mt $ h₂.rcns_unprocessed _) $ not_not.mpr h₁.self_progress, h₂.rcns_nodup⟩
 
-theorem InstExecution.ops_nodup : (e : s₁ ⇓ᵢ* s₂) → List.Nodup e.ops := by
+theorem ops_nodup : (e : s₁ ⇓ᵢ* s₂) → List.Nodup e.ops := by
   intro e
   induction e
   case refl => exact List.Nodup.nil
@@ -83,7 +43,7 @@ theorem InstExecution.ops_nodup : (e : s₁ ⇓ᵢ* s₂) → List.Nodup e.ops :
     specialize h' hd.op hm rfl
     simp [State.progress, hd.exec.ctx_adds_rcn, Context.addCurrentProcessed_mem_progress] at h'
 
-theorem InstExecution.mem_progress :
+theorem mem_progress :
   (e : s₁ ⇓ᵢ* s₂) → ∀ rcn, rcn ∈ s₂.progress ↔ rcn ∈ e.rcns ∨ rcn ∈ s₁.progress := by
   intro h rcn
   induction h
@@ -106,10 +66,10 @@ theorem InstExecution.mem_progress :
       | inr h => exact hi.mpr $ .inr $ h₁.monotonic_progress h
 
 -- Corollary of `InstExecution.mem_progress`.
-theorem InstExecution.self_progress : (e : s₁ ⇓ᵢ* s₂) → ∀ rcn ∈ e.rcns, rcn ∈ s₂.progress := 
+theorem self_progress : (e : s₁ ⇓ᵢ* s₂) → ∀ rcn ∈ e.rcns, rcn ∈ s₂.progress := 
   λ h _ hm => (h.mem_progress _).mpr $ .inl hm
   
-theorem InstExecution.eq_ctx_processed_rcns_perm : 
+theorem eq_ctx_processed_rcns_perm : 
   (e₁ : s ⇓ᵢ* s₁) → (e₂ : s ⇓ᵢ* s₂) → (s₁.ctx = s₂.ctx) → e₁.rcns ~ e₂.rcns := by
   intro h₁ h₂ he
   apply (List.perm_ext h₁.rcns_nodup h₂.rcns_nodup).mpr
@@ -130,11 +90,11 @@ theorem InstExecution.eq_ctx_processed_rcns_perm :
       rw [State.progress, ←he] at h
       exact ((h₁.mem_progress _).mp h).resolve_right hc
 
-/-theorem InstExecution.rcn_list_cons : (e : s₁ ⇓ᵢ+ s₂) → ∃ hd tl, e.rcns = hd :: tl :=
+/-theorem rcn_list_cons : (e : s₁ ⇓ᵢ+ s₂) → ∃ hd tl, e.rcns = hd :: tl :=
   (by cases · <;> simp [rcns])
 -/
 
-theorem InstExecution.to_ChangeListStep :
+theorem to_ChangeListStep :
   (e : s₁ ⇓ᵢ* s₂) → (s₁ -[e.changes]→* ⟨s₂.rtr, s₁.ctx⟩) := by
   intro e
   induction e
@@ -146,7 +106,7 @@ theorem InstExecution.to_ChangeListStep :
     exact hs
 
 /-
-theorem InstExecution.rcns_singleton (e : s₁ ⇓ᵢ+ s₂) :
+theorem rcns_singleton (e : s₁ ⇓ᵢ+ s₂) :
   (e.rcns = [rcn]) → ∃ e' : s₁ ⇓ᵢ s₂, (e'.rcn = rcn) ∧ (e = single e') := by
   intro h
   cases e
@@ -159,14 +119,14 @@ theorem InstExecution.rcns_singleton (e : s₁ ⇓ᵢ+ s₂) :
     simp [rcns] at h
     simp [rcns, h.right] at h'
 
-theorem InstExecution.mem_ops_split (e : s₁ ⇓ᵢ* s₂) :
+theorem mem_ops_split (e : s₁ ⇓ᵢ* s₂) :
   (op ∈ e.ops) → 
   ∃ (sₘ₁ : _) (sₘ₂ : _) (e₁ : s₁ ⇓ᵢ* sₘ₁) (eₘ : sₘ₁ ⇓ᵢ sₘ₂) (e₂ : sₘ₂ ⇓ᵢ* s₂), 
   (e = e₁ ++ eₘ ++ e₂) ∧ (eₘ.op = op) :=
   sorry
 -/
 
-theorem InstExecution.same_rcns_same_ops (e₁ : s ⇓ᵢ* s₁) (e₂ : s ⇓ᵢ* s₂) :
+theorem same_rcns_same_ops (e₁ : s ⇓ᵢ* s₁) (e₂ : s ⇓ᵢ* s₂) :
   (e₁.rcns ~ e₂.rcns) → (e₁.ops ~ e₂.ops) := by
   intro hp
   simp [List.perm_ext e₁.ops_nodup e₂.ops_nodup]
@@ -207,12 +167,12 @@ theorem InstExecution.same_rcns_same_ops (e₁ : s ⇓ᵢ* s₁) (e₂ : s ⇓�
   -- ... continue the list
   -/
 
-theorem InstExecution.port_change_to_op {e : s₁ ⇓ᵢ* s₂} {i : Fin e.changes.length} :
+theorem port_change_to_op {e : s₁ ⇓ᵢ* s₂} {i : Fin e.changes.length} :
   (e.changes[i].obj = .port p v) → 
   ∃ op rcn, (op ∈ e.ops) ∧ (⟨op.rcn, .port p v⟩ ∈ op.changes) ∧ (s₁.rtr.obj? .rcn op.rcn = some rcn) ∧ (p ∈ rcn.deps .out) := by
   sorry
 
-theorem InstExecution.state_change_to_op {e : s₁ ⇓ᵢ* s₂} {i : Fin e.changes.length} :
+theorem state_change_to_op {e : s₁ ⇓ᵢ* s₂} {i : Fin e.changes.length} :
   (e.changes[i].obj = .state a v) → 
   ∃ op, (op ∈ e.ops) ∧ (⟨op.rcn, .state a v⟩ ∈ op.changes) ∧ (s₁.rtr.con? .stv a = s₁.rtr.con? .rcn op.rcn) := by
   sorry
@@ -229,17 +189,17 @@ theorem Reactor.out_port_out_dep_eq_parent {rtr : Reactor} {iₚ iᵣ : ID} :
   (rtr.con? .prt iₚ = rtr.con? .rcn iᵣ) := by
   sorry
 
-theorem InstExecution.op_eq_rcn_eq {e : s₁ ⇓ᵢ* s₂} :
+theorem op_eq_rcn_eq {e : s₁ ⇓ᵢ* s₂} :
   (op₁ ∈ e.ops) → (op₂ ∈ e.ops) → (op₁.rcn = op₂.rcn) → (op₁ = op₂) := by
   sorry
 
-theorem InstExecution.ops_respect_dependencies {i₁ i₂ : Nat} : 
+theorem ops_respect_dependencies {i₁ i₂ : Nat} : 
   (e : s₁ ⇓ᵢ* s₂) →
   (e.ops[i₁]? = some op₁) → (e.ops[i₂]? = some op₂) → 
   (op₁.rcn >[s₁.rtr] op₂.rcn) → (i₁ < i₂) := by
   sorry
 
-theorem InstExecution.changes_order_to_ops_internal_order {e : s₁ ⇓ᵢ* s₂} {ic : Fin e.changes.length} {io : Nat} :
+theorem changes_order_to_ops_internal_order {e : s₁ ⇓ᵢ* s₂} {ic : Fin e.changes.length} {io : Nat} :
   (e.changes[ic].obj = c) →
   (∀ j : Fin e.changes.length, (j > ic) → e.changes[j].obj.stateValue? i = none) → 
   (op ∈ e.ops) →
@@ -247,7 +207,7 @@ theorem InstExecution.changes_order_to_ops_internal_order {e : s₁ ⇓ᵢ* s₂
   (∀ j c', (j > io) → (op.changes[j]? = some c') → c'.obj.stateValue? i = none) := by
   sorry
 
-theorem InstExecution.same_ops_ChangeListEquiv_ports {e₁ : s ⇓ᵢ* s₁} {e₂ : s ⇓ᵢ* s₂} :
+theorem same_ops_ChangeListEquiv_ports {e₁ : s ⇓ᵢ* s₁} {e₂ : s ⇓ᵢ* s₂} :
   (e₁.ops ~ e₂.ops) → (∀ i, e₁.changes.lastSome? (·.obj.portValue? i) = e₂.changes.lastSome? (·.obj.portValue? i)) := by
   intro ho i
   /-cases hc : e₁.changes.lastSome? (·.obj.portValue? i)
@@ -312,16 +272,16 @@ theorem Reactor.orderable_impure {rtr : Reactor} {i₁ i₂ : ID} :
   Reactor.Orderable rtr rcn₁ rcn₂ :=
   sorry
 
-theorem InstExecution.state_change_mem_op_rcn_eq_con? {e : s₁ ⇓ᵢ* s₂} :
+theorem state_change_mem_op_rcn_eq_con? {e : s₁ ⇓ᵢ* s₂} :
   (op ∈ e.ops) → (⟨op.rcn, .state i v⟩ ∈ op.changes) → 
   (s₁.rtr.con? .stv i = s₁.rtr.con? .rcn op.rcn)
   := sorry
 
-theorem InstExecution.state_change_mem_op_rcn_impure {e : s₁ ⇓ᵢ* s₂} :
+theorem state_change_mem_op_rcn_impure {e : s₁ ⇓ᵢ* s₂} :
   (op ∈ e.ops) → (⟨op.rcn, .state i v⟩ ∈ op.changes) →
   ∃ rcn, (s₁.rtr.obj? .rcn op.rcn = some rcn) ∧ (¬rcn.isPure) := sorry
 
-theorem InstExecution.same_ops_ChangeListEquiv_state {e₁ : s ⇓ᵢ* s₁} {e₂ : s ⇓ᵢ* s₂} :
+theorem same_ops_ChangeListEquiv_state {e₁ : s ⇓ᵢ* s₁} {e₂ : s ⇓ᵢ* s₂} :
   (e₁.ops ~ e₂.ops) → (∀ i, e₁.changes.lastSome? (·.obj.stateValue? i) = e₂.changes.lastSome? (·.obj.stateValue? i)) := by
   intro ho i
   have ⟨v₁, hc₁⟩ : ∃ v, e₁.changes.lastSome? (·.obj.stateValue? i) = some v := sorry
@@ -388,11 +348,11 @@ theorem InstExecution.same_ops_ChangeListEquiv_state {e₁ : s ⇓ᵢ* s₁} {e�
     -- Thus (wlog. assuming op₁ must appear before op₂) e₁.ops must also contain op₂ (by `ho`) somewhere after op₁. 
     -- Thus the assumption hj₂ is false.
 
-theorem InstExecution.same_ops_ChangeListEquiv_actions {e₁ : s ⇓ᵢ* s₁} {e₂ : s ⇓ᵢ* s₂} :
+theorem same_ops_ChangeListEquiv_actions {e₁ : s ⇓ᵢ* s₁} {e₂ : s ⇓ᵢ* s₂} :
   (e₁.ops ~ e₂.ops) → (∀ i t, e₁.changes.filterMap (·.obj.actionValue? i t) = e₂.changes.filterMap (·.obj.actionValue? i t)) := by
   sorry
 
-theorem InstExecution.same_rcns_ChangeListEquiv {e₁ : s ⇓ᵢ* s₁} {e₂ : s ⇓ᵢ* s₂} : 
+theorem same_rcns_ChangeListEquiv {e₁ : s ⇓ᵢ* s₁} {e₂ : s ⇓ᵢ* s₂} : 
   (e₁.rcns ~ e₂.rcns) → (e₁.changes ⋈ e₂.changes) := by
   intro hr
   have ho := e₁.same_rcns_same_ops e₂ hr
@@ -402,7 +362,7 @@ theorem InstExecution.same_rcns_ChangeListEquiv {e₁ : s ⇓ᵢ* s₁} {e₂ : 
     actions := same_ops_ChangeListEquiv_actions ho
   }
 
-protected theorem InstExecution.deterministic : 
+protected theorem deterministic : 
   (s ⇓ᵢ* s₁) → (s ⇓ᵢ* s₂) → (s₁.ctx = s₂.ctx) → s₁ = s₂ := by
   intro e₁ e₂ hc
   refine State.ext _ _ ?_ hc
@@ -411,6 +371,55 @@ protected theorem InstExecution.deterministic :
   injection e₁.to_ChangeListStep.equiv_changes_eq_result e₂.to_ChangeListStep he
   assumption
     
-theorem InstExecution.trivial_eq [State.Trivial s₁] : (s₁ ⇓ᵢ* s₂) → s₁ = s₂
+
+
+
+
+
+theorem trivial_eq [State.Trivial s₁] : (s₁ ⇓ᵢ* s₂) → s₁ = s₂
   | refl => rfl
   | trans e _ => absurd (inferInstanceAs s₁.Trivial) e.not_Trivial 
+
+theorem tag_eq : (s₁ ⇓ᵢ* s₂) → s₁.tag = s₂.tag
+  | refl => rfl
+  | trans e e' => e.exec.preserves_tag.trans e'.tag_eq
+
+-- TODO: To you need this for `ctx_eq`?
+theorem preserves_ctx_past_future :
+  (s₁ ⇓ᵢ* s₂) → ∀ g, g ≠ s₁.tag → s₁.ctx.processedRcns g = s₂.ctx.processedRcns g := by
+  intro h g hg
+  induction h
+  case refl => rfl
+  case trans s₁ _ sₘ he _ hi =>
+    rw [InstExecution.tag_eq $ trans he refl] at hg
+    exact (he.exec.preserves_ctx_past_future _ hg).trans $ hi hg
+    
+  /-
+  
+  ext1; ext1 g
+  have hc₁₂ := hc₁.rcns_eq hc₂
+  cases hc₁ with | mk e₁ hc₁ => 
+  cases hc₂ with | mk e₂ hc₂ => 
+  by_cases hg : g = s.tag
+  case pos => 
+    have h₁ := hc₁ |> Option.some_inj.mpr
+    have h₂ := hc₂ |> Option.some_inj.mpr
+    rw [Context.progress_def] at h₁ h₂
+    simp only [←e₁.tag_eq, ←e₂.tag_eq, ←hg] at h₁ h₂
+    simp only [h₁, h₂, hc₁₂]
+  case neg => simp only [←e₁.preserves_ctx_past_future g hg, e₂.preserves_ctx_past_future g hg]
+  -/
+
+theorem ctx_eq (e : s₁ ⇓ᵢ* s₂) : s₂.ctx = s₁.ctx.process e.rcns :=
+  sorry
+
+theorem mem_rcns_iff (e : s₁ ⇓ᵢ* s₂) (rcn : ID) : 
+  rcn ∈ e.rcns ↔ (rcn ∈ s₂.progress ∧ rcn ∉ s₁.progress) := by
+  sorry
+
+theorem preserves_rcns {i : ID} : (s₁ ⇓ᵢ* s₂) → (s₁.rtr.obj? .rcn i = s₂.rtr.obj? .rcn i)
+  | refl => rfl
+  | trans e e' => e.exec.preserves_rcns ▸ e'.preserves_rcns
+
+end InstExecution
+end Execution
