src/ReactorModel/Determinism/Trivial.lean
@@ -1,0 +1,43 @@
+import ReactorModel.Determinism.ExecutionStep
+
+namespace Execution
+
+instance AdvanceTag.preserves_Trivial [State.Trivial s₁] {e : s₁ ⇓- s₂} : State.Trivial s₂ :=
+  match e with | ⟨_, _⟩ => inferInstance
+
+instance ClosedExecution.preserves_Trivial [State.Trivial s₁] {e : s₁ ⇓| s₂} : 
+    State.Trivial s₂ where
+  trivial := e.preserves_rcns ▸ State.Trivial.trivial
+
+theorem ClosedExecution.trivial_eq [State.Trivial s₁] (e : s₁ ⇓| s₂) : s₁ = s₂ :=
+  e.exec.trivial_eq
+
+instance Step.preserves_Trivial [State.Trivial s₁] : (s₁ ⇓ s₂) → State.Trivial s₂
+  | close e => e.preserves_Trivial
+  | advance a => a.preserves_Trivial
+
+inductive AdvanceTag.RTC : State → State → Type
+  | refl : RTC s s
+  | trans : (s₁ ⇓- s₂) → (RTC s₂ s₃) → RTC s₁ s₃   
+
+theorem AdvanceTag.RTC.deterministic 
+  (a₁ : AdvanceTag.RTC s s₁) (a₂ : AdvanceTag.RTC s s₂) (ht : s₁.tag = s₂.tag) : s₁ = s₂ := by
+  induction a₁ <;> cases a₂
+  case refl.refl                       => rfl
+  case' refl.trans a _, trans.refl _ a => exact absurd ht a.tag_ne
+  case trans.trans a₁ _ hi _ a₂ c₂     => exact hi (a₂.determinisic a₁ ▸ c₂) ht
+
+def to_AdvanceTagRTC [State.Trivial s₁] : (s₁ ⇓* s₂) → AdvanceTag.RTC s₁ s₂
+  | refl => .refl
+  | step (.advance a) e' => 
+    have := a.preserves_Trivial -- TODO: Make this work via type class inference.
+    .trans a e'.to_AdvanceTagRTC
+  | step (.close e) e' => 
+    have := e.preserves_Trivial -- TODO: Make this work via type class inference.
+    e.trivial_eq ▸ e'.to_AdvanceTagRTC
+
+theorem trivial_deterministic [trivial : State.Trivial s] 
+    (e₁ : s ⇓* s₁) (e₂ : s ⇓* s₂) (ht : s₁.tag = s₂.tag) : s₁ = s₂ :=
+  e₁.to_AdvanceTagRTC.deterministic e₂.to_AdvanceTagRTC ht
+
+end Execution
